withtop/Proofs/semantics/SemanticsBiRed.v
@@ -5,36 +5,6 @@ Require Import LibLN.
 Require Import STLCNew.
 Require Import CoherenceBasicBDNew.
 
-
-Inductive typing : env PTyp -> PExp -> PTyp -> Prop :=
-  | TyVar' : forall Gamma x ty,
-               ok Gamma ->
-               binds x ty Gamma ->
-               WFTyp ty ->
-               typing Gamma (PFVar x) ty
-  | TyLit' : forall Gamma i,
-               ok Gamma ->
-               typing Gamma (PLit i) PInt
-  | TyLam' : forall L Gamma t A B,
-               (forall x, x \notin L ->
-                     typing (Gamma & x ~ A) (open_source t (PFVar x)) B) ->
-               WFTyp A ->
-               typing Gamma (PLam t) (Fun A B)
-  | TyApp' : forall Gamma A B t1 t2,
-               typing Gamma t1 (Fun A B) ->
-               typing Gamma t2 A ->
-               typing Gamma (PApp t1 t2) B
-  | TyMerge' : forall Gamma A B t1 t2,
-                 typing Gamma t1 A ->
-                 typing Gamma t2 B ->
-                 OrthoS A B ->
-                 typing Gamma (PMerge t1 t2) (And A B)
-  | TySub' : forall Gamma t A B,
-               typing Gamma t A ->
-               Sub A B ->
-               WFTyp B ->
-               typing Gamma t B.
-
 Inductive VChk : PExp -> PTyp -> Prop :=
   | VLam : forall A B t, VChk (PLam t) (Fun A B).
 
@@ -46,40 +16,6 @@ Inductive VInf : PExp -> PTyp -> Prop :=
   | VAnn : forall v A, VChk v A -> VInf (PAnn v A) A. 
 
 Hint Constructors VChk VInf.
-
-Inductive bidityping : env PTyp -> PExp -> Dir -> PTyp -> Prop :=
-  | ATyVar' : forall Gamma x ty,
-                ok Gamma ->
-                binds x ty Gamma ->
-                WFTyp ty ->
-                bidityping Gamma (PFVar x) Inf ty
-  | ATyLit' : forall Gamma (x : nat),
-                ok Gamma ->
-                bidityping Gamma (PLit x) Inf PInt
-  | ATyApp' : forall Gamma (A B : PTyp) (t1 t2 : PExp),
-                bidityping Gamma t1 Inf (Fun A B) ->
-                bidityping Gamma t2 Chk A ->
-                bidityping Gamma (PApp t1 t2) Inf B
-  | ATyMerge' : forall Gamma (A B : PTyp) (t1 t2 : PExp),
-                  bidityping Gamma t1 Inf A ->
-                  bidityping Gamma t2 Inf B ->
-                  OrthoS A B ->
-                  bidityping Gamma (PMerge t1 t2) Inf (And A B)
-  | ATyAnnCT' : forall Gamma (t1 : PExp) (A : PTyp),
-                  bidityping Gamma t1 Chk A ->
-                  bidityping Gamma (PAnn t1 A) Inf A
-  | ATyLam' : forall L Gamma 
-                (t : PExp) (A B : PTyp),
-                (forall x, x \notin L ->
-                      bidityping (Gamma & x ~ A) (open_source t (PFVar x)) Chk B) ->
-                WFTyp A ->
-                bidityping Gamma (PLam t) Chk (Fun A B)
-  | ATySub' : forall Gamma (t : PExp) 
-                (A B : PTyp) C,
-                bidityping Gamma t Inf A ->
-                sub A B C ->
-                WFTyp B ->
-                bidityping Gamma t Chk B.
 
 Definition value (v : PExp) := exists A, VInf v A.
 
@@ -141,114 +77,14 @@ Inductive bired : PExp -> PExp -> Prop :=
   | Red_Ann3 : forall v A, VInf v A ->
                       bired (PAnn v A) v.
 
-Hint Constructors typing bidityping WFTyp subred bired.
-
-(** Soundness and Completeness wrt to the elaborating biditypecheker **)
-
-
-Theorem has_type_source_alg_rename :
-  forall L Gamma A B t1 c m y,
-    has_type_source_alg (Gamma & y ~ A) (open_source t1 (PFVar y)) B m 
-                        (open c (STFVar y)) ->
-    (forall x, x \notin L ->
-          has_type_source_alg (Gamma & x ~ A) (open_source t1 (PFVar x)) B m
-                              (open c (STFVar x))).
-Proof.
-  intros.
-  (* subst_typ_source_intro *)
-Admitted.
-  
-Theorem soundness : forall Gamma e A m, bidityping Gamma e A m -> has_ty Gamma e A m.
-Proof.
-  intros Gamma e A m H; unfold has_ty.
-  induction H; destruct_conjs; eauto.
-  - pick_fresh x.
-    assert (Ha : x \notin L) by autos*.
-    destruct (H0 _ Ha) as [c H2].
-    exists (STLam' c).
-    apply_fresh ATyLam as z; auto.
-    apply has_type_source_alg_rename with (L := L) (y := x).
-    admit. (* missing the good old renaming lemma... *)
-    autos*.
-Admitted.
-    
-Theorem completeness :
-  forall Gamma A m d e, has_type_source_alg Gamma e A m d -> bidityping Gamma e A m.
-Proof. intros Gamma A m d e H; induction H; eauto; destruct m; auto. Qed.
-
-Hint Resolve soundness completeness.
-
-(** Some necessary properties about bidityping, which are lifted from 
-    the elaborated version **)
-
-Theorem bityping_ok : forall Gamma t A m, bidityping Gamma t m A -> ok Gamma.
-Proof.
-  intros; apply soundness in H as [c H]; eapply typing_alg_ok_env; eauto.
-Qed.
-  
-Theorem bityping_wf : forall Gamma t A m, bidityping Gamma t m A -> WFTyp A.
-Proof.
-  intros; apply soundness in H as [c H]; eapply typing_wf_source_alg; eauto.
-Qed.
-
-Theorem bityping_term : forall Gamma e A m, bidityping Gamma e m A -> PTerm e.
-Proof.
-  intros; apply soundness in H as [c H]; eapply type_correct_alg_terms; eauto.
-Qed.
-
-Theorem bityping_weaken:
-  forall G E F t T dir, bidityping (E & G) t dir T ->
-                   ok (E & F & G) ->
-                   bidityping (E & F & G) t dir T.
-Proof.
-  intros; apply soundness in H as [c H].
-  lets* Ha : typing_weaken_alg H.
-Qed.
-
-Lemma typing_strengthen_alg : forall z U E F t T d c,
-  z \notin (fv_source t) ->
-  has_type_source_alg (E & z ~ U & F) t T d c ->
-  has_type_source_alg (E & F) t T d c.
-Proof.
-  intros.
-  remember (E & z ~ U & F).
-  gen Heqe. gen F. 
-  induction H0; intros; substs*; simpls*.
-  - apply* ATyVar; simpls*; apply* binds_remove.
-  - apply_fresh* ATyLam as x.
-    apply_ih_bind* H1; apply* fv_source_distr2; simpls*.
-Qed.
-
-Theorem bityping_strengthen:
-  forall z U E F e dir A,
-    z \notin (fv_source e) ->
-    bidityping (E & z ~ U & F) e dir A ->
-    bidityping (E & F) e dir A.
-Proof.
-  intros z U E F e dir A H1 H2; apply soundness in H2 as [c H2].
-  lets* Ha : typing_strengthen_alg H1 H2.
-Qed.
+Hint Constructors WFTyp subred bired.
 
 (* We didn't prove this before?! See: Pfenning *)
 Theorem sub_trans : forall A B, Sub A B -> forall C, Sub B C -> Sub A C. Admitted.
 
-Hint Resolve bityping_ok bityping_wf bityping_term bityping_weaken
-     reflex sub_trans.
+Hint Resolve reflex sub_trans.
 Hint Unfold Sub.
 
-(*
-Theorem bityping_ann_sub :
-  forall Gamma t A B m1 m2, bidityping Gamma (PAnn m1 t A) m2 B -> Sub A B.
-Proof. intros Gamma t A B m1 m2 Htyping; dependent induction Htyping; eauto. Qed.
-
-Theorem bityping_ann :
-  forall Gamma t A B m1 m2, bidityping Gamma (PAnn m1 t A) B m2 -> bidityping Gamma t Chk A.
-Proof. intros Gamma t A B m1 m2 Htyping; dependent induction Htyping; eauto. Qed.
-*)
-
-(** Properties mixing "Sub", "In" and the type-system. **)
-
-(*Hint Resolve bityping_ann_sub bityping_ann.*)
 Hint Unfold erase.
 
 Theorem VInf_bityping_eq :
@@ -291,52 +127,6 @@ Qed.
 
 Hint Resolve bityping_inf_chk.
 
-(** Defining body. (getting ready for subject reduction) **)
-
-Definition body_bityping Gamma t A B m :=
-  exists L, forall x, x \notin L ->
-            bidityping (Gamma & x ~ A) (open_source t (PFVar x)) m B.
-
-Hint Unfold body_bityping.
-
-Lemma abs_to_body_bityping : forall A B e Gamma m, 
-  bidityping Gamma (PLam e) m (Fun A B) -> body_bityping Gamma e A B m.
-Proof. intros; inversion H; subst; eauto; inversion H0. Qed.
-
-Lemma bityping_subst : forall Gamma A B e u m x,
-                         binds x B Gamma ->
-                         bidityping Gamma e m A ->
-                         bidityping Gamma u Inf B ->
-                         bidityping Gamma (subst_source x u e) m A.
-Proof.
-  intros Gamma A B e u m x HIn H1 H2.
-  induction H1; simpl; eauto.
-  - case_var*.
-    assert (Ha : B = ty) by (eapply binds_func; eauto). now subst.
-  - apply_fresh ATyLam' as x; auto.
-    rewrite subst_source_open_var; eauto.
-    apply H0; autos*.
-    rewrite <- concat_empty_r with (E := (Gamma & y ~ A)).
-    apply bityping_weaken; rewrite concat_empty_r; autos*.
-Qed.
-
-Lemma open_body_bityping :
-  forall e A B u Gamma m, body_bityping Gamma e A B m -> bidityping Gamma u Inf A ->
-                 bidityping Gamma (open_source e u) m B.
-Proof.
-  intros e A B u Gamma m H1 H2; destruct H1. pick_fresh y.
-  assert (Ha : y \notin x) by autos*; apply H in Ha.
-  rewrite <- concat_empty_r with (E := Gamma).
-  eapply bityping_strengthen with (z := y) (U := A).
-  apply fv_source_distr2; autos*.
-  rewrite concat_empty_r.
-  rewrite subst_source_intro with (x := y); autos*.
-  apply bityping_subst with (B := A); autos*.
-  rewrite <- concat_empty_r with (E := (Gamma & y ~ A)).
-  apply bityping_weaken; rewrite concat_empty_r; autos*.
-Qed.
-
-
 (** Theorem 1. Subject reduction **)
 
 Theorem subject_reduction_sub :
@@ -355,7 +145,7 @@ Proof.
     apply ATySub' with (A := Fun C D) (C := x); eauto.
     apply ATyAnnCT'.
     assert (Ha : WFTyp (Fun A0 B)) by
-        (now assert (Ha := bityping_wf _ _ _ _ Htyping); inversion Ha).
+        (now assert (Ha := bityping_wf Htyping); inversion Ha).
     inverts Ha.
     apply_fresh ATyLam' as x; auto.
     unfold open_source; simpl.
